intermediate/Veritas.Intermediate.TSLog.fst
@@ -1,54 +1,142 @@
 module Veritas.Intermediate.TSLog
+open FStar.Calc
+module VG = Veritas.Intermediate.Global
+module VT = Veritas.Intermediate.Thread
 
-let create (#vcfg:_) (gl: verifiable_log vcfg): (itsl:its_log vcfg{g_logS_of itsl == gl}) = admit()
+#push-options "--query_stats --max_fuel 0 --max_ifuel 0 --z3rlimit_factor 4"
+let lemma_prefix_clock_sorted #vcfg 
+                              (itsl: its_log vcfg) 
+                              (i:nat{i <= I.length itsl})
+  : Lemma
+    (requires
+      verifiable (I.prefix itsl i))
+    (ensures
+      clock_sorted (I.prefix itsl i))
+  = assert (clock_sorted itsl);
+    let itsl' = I.prefix itsl i in
+    let aux (t0 t1:I.seq_index itsl')
+      : Lemma (requires t0 <= t1)
+              (ensures clock itsl' t0 `ts_leq` clock itsl' t1)
+              [SMTPat(clock itsl' t0 `ts_leq` clock itsl' t1)]
+      = assert (clock itsl t0 `ts_leq` clock itsl t1);
+        lemma_i2s_map_prefix itsl i t0;
+        lemma_i2s_map_prefix itsl i t1;
+        I.lemma_prefix_index itsl i t0;
+        I.lemma_prefix_index itsl i t1;
+        I.per_thread_prefix itsl i;
+        calc (==) {
+         clock itsl' t0;
+          == {}
+         clock (I.prefix itsl i) t0;
+          == {}
+         VG.clock (g_logS_of itsl') (i2s_map itsl' t0);
+          == {}
+         VG.clock (g_logS_of itsl') (i2s_map itsl t0);
+        }
+    in
+    ()
 
-let lemma_prefix_verifiable (#vcfg:_) (itsl: its_log vcfg) (i:nat{i <= I.length itsl}):
-  Lemma (ensures (verifiable (I.prefix itsl i) /\ clock_sorted (I.prefix itsl i))) = admit()
+let lemma_prefix_verifiable #vcfg (itsl: its_log vcfg) (i:nat{i <= I.length itsl})
+  : Lemma
+    (ensures
+      verifiable (I.prefix itsl i) /\
+      clock_sorted (I.prefix itsl i))
+  = assert (verifiable itsl);
+    assert (clock_sorted itsl);
+    let ss = g_logS_of itsl in
+    let itsl' = I.prefix itsl i in
+    let ss' = g_logS_of itsl' in
+    assert (Seq.length ss = Seq.length ss');
+    let aux (tid:SA.seq_index ss)
+      : Lemma (VT.verifiable (thread_log ss' tid))
+              [SMTPat (thread_log ss' tid)]
+      = let tl = thread_log ss tid in
+        assert (VT.verifiable tl);
+        I.per_thread_prefix itsl i;
+        let tl' = thread_log ss' tid in
+        VT.verifiable_implies_prefix_verifiable tl (Seq.length (snd tl'))
+    in
+    lemma_prefix_clock_sorted itsl i
 
-let lemma_verifier_thread_state_extend (#vcfg:_) (ils: its_log vcfg) (i: I.seq_index ils):
-  Lemma (ensures (thread_state_post ils i == IntV.verify_step (thread_state_pre ils i) (I.index ils i))) = admit()
+let create (#vcfg:_) (gl: verifiable_log vcfg)
+  : itsl:its_log vcfg{g_logS_of itsl == gl}
+  = admit()
 
-let lemma_slot_is_merkle_points_to (#vcfg:_) (ils: its_log vcfg) (i: I.seq_index ils):
-  Lemma (ensures (slot_points_to_is_merkle_points_to (IntV.thread_store (thread_state_pre ils i)))) = admit()
+#push-options "--max_fuel 1"
+let lemma_verifier_thread_state_extend (#vcfg:_) (itsl: its_log vcfg) (i: I.seq_index itsl)
+  : Lemma (ensures (thread_state_post itsl i ==
+                    IntV.verify_step (thread_state_pre itsl i) (I.index itsl i))) 
+  = let tid = thread_id_of itsl i in
+    let itsl_i = I.prefix itsl i in
+    let vlog_tid = Seq.index (s_seq itsl_i) tid in
+    let itsl_i' = I.prefix itsl (i + 1) in
+    let vlog_tid' = Seq.index (s_seq itsl_i') tid in
+    I.lemma_prefix_snoc itsl i;
+    assert (vlog_tid' `Seq.equal` Seq.snoc vlog_tid (I.index itsl i));
+    assert (prefix vlog_tid' (Seq.length vlog_tid' - 1) `Seq.equal` vlog_tid);
+    ()
+#pop-options
+
+let lemma_slot_is_merkle_points_to (#vcfg:_) (ils: its_log vcfg) (i: I.seq_index ils)
+  : Lemma (ensures (slot_points_to_is_merkle_points_to (IntV.thread_store (thread_state_pre ils i))))
+  = admit()
+
+#push-options "--max_fuel 2 --max_ifuel 1 --z3rlimit_factor 4"
+let int_add_sub_log #vcfg (il:its_log vcfg { IntAdd? (IL?.prf il) })
+  : its_log vcfg
+  = let IL s ss prf = il in
+    let IntAdd s' ss' prf' = prf in
+    let il' = IL s' ss' prf' in
+    assert(Seq.equal ss (append1 ss' Seq.empty));
+    assert (forall (tid:Veritas.SeqAux.seq_index ss'). IntG.thread_log ss' tid == IntG.thread_log ss tid);
+    I.i2s_map_int_add il';
+    assert (forall (i:I.seq_index il'). clock il' i == clock il i);      
+    assert (clock_sorted il');      
+    il'
+
+let int_extend_sub_log #vcfg (il:its_log vcfg { IntExtend? (IL?.prf il) })
+  : il':its_log vcfg{il' == I.prefix il (I.length il - 1)} 
+  = let IL s ss prf = il in
+    let IntExtend s0 ss0 prf x i = prf in
+    let il' = IL _ _ prf in
+    I.hprefix_extend _ _ prf x i;      
+    let n' = I.length il - 1 in
+    lemma_prefix_verifiable il' n';
+    assert(il' == I.prefix il n');
+    il'
+
+let int_extend_logK_entry #vcfg (il:its_log vcfg { IntExtend? (IL?.prf il) })
+  : logK_entry
+  = let IL s ss prf = il in
+    let IntExtend s0 ss0 prf x i = prf in
+    let n' = I.length il - 1 in
+    let vss_pre = thread_state_pre il n' in
+    assert (I.index il n' == x);
+    let ek = IntV.to_logK_entry vss_pre x in
+    ek
 
 let rec to_logk_aux #vcfg (il:its_log vcfg) 
   : Tot (sil:SpecTS.il_vlog { same_shape il sil })
         (decreases (I.IL?.prf il))
-  = admit()
-
-(*
-  let IL s ss prf = il in
+  = let IL s ss prf = il in
     match prf with
     | IntEmpty -> 
       IL _ _ IntEmpty
 
     | IntAdd s' ss' prf ->
-      let il' = IL s' ss' prf in
-      assert(Seq.equal ss (append1 ss' Seq.empty));
-      assert (forall (tid:Veritas.SeqAux.seq_index ss'). IntG.thread_log ss' tid == IntG.thread_log ss tid);
-      I.i2s_map_int_add il';
-      assert (forall (i:I.seq_index il'). clock il' i == clock il i);      
-      assert (clock_sorted il');      
+      let il' = int_add_sub_log il in
       let IL _ _ prf = to_logk_aux il' in
       let res = IL _ _ (IntAdd _ _ prf) in
       res      
 
     | IntExtend s0 ss0 prf x i ->
-      let il' = IL _ _ prf in
-      I.hprefix_extend _ _ prf x i;      
       let n' = I.length il - 1 in
-      lemma_prefix_verifiable il' n';
-      assert(il' == I.prefix il n');
-      let vss_pre = thread_state_pre il n' in
-      let vss_post = thread_state_post il n' in
-      let es = I.index il n' in
-      assert(vss_post == IntV.verify_step vss_pre es);
-      let ek = IntV.to_logK_entry vss_pre es in
-      
+      let il' = int_extend_sub_log il in
+      let ek = int_extend_logK_entry il in
       let IL _ ss0k prfk = to_logk_aux il' in 
       let res = I.IntExtend _ _ prfk ek i in
       IL _ _ res      
-*)
+#pop-options
 
 let to_logk (#vcfg:_) (il:its_log vcfg) 
   : Tot (sil:SpecTS.il_vlog { same_shape il sil }) = 
@@ -61,9 +149,43 @@ let lemma_to_logk_thread_count (#vcfg:_) (il:its_log vcfg)
   : Lemma (ensures thread_count il = SpecTS.thread_count (to_logk il))
   = ()
 
-let lemma_to_logk_thread_id_of (#vcfg:_) (il:its_log vcfg) (i:I.seq_index il)
-  : Lemma (ensures thread_id_of il i == SpecTS.thread_id_of (to_logk il) i)
+#push-options "--ifuel 1,1 --fuel 1,1"
+
+let lemma_to_logk_prefix_commute_aux (#vcfg:_) (il:its_log vcfg) (i:nat{i <= I.length il})
+  : Lemma (to_logk (I.prefix il i) == I.prefix (to_logk il) i)
   = admit()
+
+let rec lemma_to_logk_thread_id_of_aux (#vcfg:_) (il:its_log vcfg) (i:I.seq_index il)
+  : Lemma (ensures thread_id_of il i == SpecTS.thread_id_of (to_logk il) i)
+          (decreases IL?.prf il)
+  = let IL s ss prf = il in
+    match prf with
+    | IntEmpty -> ()
+
+    | IntAdd s' ss' prf' ->
+      let il' = int_add_sub_log il in
+      lemma_to_logk_thread_id_of_aux il' i; 
+      I.i2s_map_int_add il';
+      I.i2s_map_int_add (to_logk il');
+      assert (thread_id_of il' i == thread_id_of il i);
+      assert (SpecTS.thread_id_of (to_logk il) i == SpecTS.thread_id_of (to_logk il') i)
+
+    | IntExtend s0 ss0 prf x j ->
+      let il' = int_extend_sub_log il in
+      if i = I.length il - 1 
+      then (
+        i2s_map_int_extend _ _ prf x j i;
+        assert (thread_id_of il i == j);
+        let lk' = to_logk il' in
+        let lk = to_logk il in
+        i2s_map_int_extend _ _ (IL?.prf lk') (int_extend_logK_entry il) j i
+      )
+      else (
+        lemma_to_logk_thread_id_of_aux il' i;
+        lemma_to_logk_prefix_commute_aux il (I.length il - 1);
+        I.lemma_i2s_map_prefix il (I.length il - 1) i;
+        I.lemma_i2s_map_prefix (to_logk il) (I.length il - 1) i
+      )
 
 let lemma_to_logk_prefix_commute (#vcfg:_) (il:its_log vcfg) (i:nat{i <= I.length il})
   : Lemma (to_logk (I.prefix il i) == I.prefix (to_logk il) i)
